Move the FFI wrappers out of TestAPI into FFI
No code changes - just moved to a different source file.

src/tls/test/FFIRegister.ml
@@ -1,5 +1,5 @@
-let _ = Callback.register "MITLS_FFI_Config" TestAPI.ffiConfig;
-        Callback.register "MITLS_FFI_Connect"  TestAPI.ffiConnect;
-        Callback.register "MITLS_FFI_Send" TestAPI.ffiSend;
-        Callback.register "MITLS_FFI_Recv" TestAPI.ffiRecv;
+let _ = Callback.register "MITLS_FFI_Config" FFI.ffiConfig;
+        Callback.register "MITLS_FFI_Connect"  FFI.ffiConnect;
+        Callback.register "MITLS_FFI_Send" FFI.ffiSend;
+        Callback.register "MITLS_FFI_Recv" FFI.ffiRecv;
         
